<?xml version="1.0" encoding="UTF-8"?>
<exercises xmlns:xi="http://www.w3.org/2001/XInclude" xml:id="exercises_sec-logic">

  <exercise>
    <statement>
      <p>
        Consider the statement about a party,
        <q>If it's your birthday or there will be cake,
        then there will be cake.</q>

        <ol>
          <li>
            <p>
              Translate the above statement into symbols.
              Clearly state which statement is <m>P</m> and which is <m>Q</m>.
            </p>
          </li>

          <li>
            <p>
              Make a truth table for the statement.
            </p>
          </li>

          <li>
            <p>
              Assuming the statement is true, what
              (if anything)
              can you conclude if there will be cake?
            </p>
          </li>

          <li>
            <p>
              Assuming the statement is true, what
              (if anything)
              can you conclude if there will not be cake?
            </p>
          </li>

          <li>
            <p>
              Suppose you found out that the statement was a lie.
              What can you conclude?
            </p>
          </li>
        </ol>
      </p>
    </statement>
    <solution>
      <p>
        <ol>
          <li>
            <m>P</m>: it's your birthday; <m>Q</m>:
            there will be cake. <m>(P \vee Q) \imp Q</m>
          </li>

          <li>
            <p>
              Hint: you should get three T's and one F.
            </p>
          </li>

          <li>
            <p>
              Only that there will be cake.
            </p>
          </li>

          <li>
            <p>
              It's NOT your birthday!
            </p>
          </li>

          <li>
            <p>
              It's your birthday, but the cake is a lie.
            </p>
          </li>
        </ol>
      </p>
    </solution>
  </exercise>

  <exercise>
    <statement>
      <p>
        Make a truth table for the statement <m>(P \vee Q) \imp (P \wedge Q)</m>.
      </p>
    </statement>
    <solution>
      <sidebyside>

        <tabular halign="center">
          <col right="minor"/>
          <col right="medium"/>
          <col/>
          <row bottom="minor">
            <cell><m>P</m></cell>
            <cell><m>Q</m></cell>
            <cell><m>(P \vee Q) \imp (P \wedge Q)</m></cell>
          </row>
          <row>
            <cell>T</cell>
            <cell>T</cell>
            <cell>T</cell>
          </row>
          <row>
            <cell>T</cell>
            <cell>F</cell>
            <cell>F</cell>
          </row>
          <row>
            <cell>F</cell>
            <cell>T</cell>
            <cell>F</cell>
          </row>
          <row>
            <cell>F</cell>
            <cell>F</cell>
            <cell>T</cell>
          </row>
        </tabular>

      </sidebyside>
    </solution>
  </exercise>

  <exercise>
    <statement>
      <p>
        Make a truth table for the statement <m>\neg P \wedge (Q \imp P)</m>.
        What can you conclude about <m>P</m> and <m>Q</m> if you know the statement is true?
      </p>
    </statement>
    <solution>
      <sidebyside>

        <tabular halign="center">
          <col right="minor"/>
          <col right="medium"/>
          <col/>
          <row bottom="minor">
            <cell><m>P</m></cell>
            <cell><m>Q</m></cell>
            <cell><m>\neg P \wedge (Q \imp P)</m></cell>
          </row>
          <row>
            <cell>T</cell>
            <cell>T</cell>
            <cell>F</cell>
          </row>
          <row>
            <cell>T</cell>
            <cell>F</cell>
            <cell>F</cell>
          </row>
          <row>
            <cell>F</cell>
            <cell>T</cell>
            <cell>F</cell>
          </row>
          <row>
            <cell>F</cell>
            <cell>F</cell>
            <cell>T</cell>
          </row>
        </tabular>

      </sidebyside>

      <p>
        If the statement is true, then both <m>P</m> and <m>Q</m> are false.
      </p>
    </solution>
  </exercise>

  <exercise>
    <statement>
      <p>
        Make a truth table for the statement <m>\neg P \imp (Q \wedge R)</m>.
      </p>
    </statement>
    <hint>
      <p>
        Like above, only now you will need 8 rows instead of just 4.
      </p>
    </hint>
  </exercise>

  <exercise>
    <statement>
      <p>
        Determine whether the following two statements are logically equivalent:
        <m>\neg(P \imp Q)</m> and <m>P \wedge \neg Q</m>.
        Explain how you know you are correct.
      </p>
    </statement>
    <solution>
      <p>
        Make a truth table for each and compare.
        The statements are logically equivalent.
      </p>
    </solution>
  </exercise>

  <exercise>
    <statement>
      <p>
        Are the statements <m>P \imp (Q\vee R)</m> and
        <m>(P \imp Q) \vee (P \imp R)</m> logically equivalent?
      </p>
    </statement>
  </exercise>

  <exercise>
    <statement>
      <p>
        Simplify the following statements
        (so that negation only appears right before variables).

        <ol>
          <li><m>\neg(P \imp \neg Q)</m>.</li>

          <li>
            <m>(\neg P \vee \neg Q) \imp \neg (\neg Q \wedge R)</m>.
          </li>

          <li>
            <m>\neg((P \imp \neg Q) \vee \neg (R \wedge \neg R))</m>.
          </li>

          <li>
            <p>
              It is false that if Sam is not a man then Chris is a woman,
              and that Chris is not a woman.
            </p>
          </li>
        </ol>
      </p>
    </statement>
    <answer>
      <p>
        <ol>
          <li><m>P \wedge Q</m>.</li>

          <li>
            <m>(\neg P \vee \neg R) \imp (Q \vee \neg R)</m> or,
            replacing the implication with a disjunction first:
            <m>(P \wedge Q) \vee (Q \vee \neg R)</m>.
          </li>

          <li>
            <p>
              <m>(P \wedge Q) \wedge (R \wedge \neg R)</m>.
              This is necessarily false,
              so it is also equivalent to <m>P \wedge \neg P</m>.
            </p>
          </li>

          <li>
            <p>
              Either Sam is a woman and Chris is a man, or Chris is a woman.
            </p>
          </li>
        </ol>
      </p>
    </answer>
  </exercise>

  <exercise>
    <statement>
      <p>
        Use De Morgan's Laws,
        and any other logical equivalence facts you know to simplify the following statements.
        Show all your steps.
        Your final statements should have negations only appear directly next to the sentence variables or predicates (<m>P</m>,
        <m>Q</m>, <m>E(x)</m>, etc.), and no double negations.
        It would be a good idea to use only conjunctions,
        disjunctions, and negations.

        <ol>
          <li>
            <m>\neg((\neg P \wedge Q) \vee \neg(R \vee \neg S))</m>.
          </li>

          <li>
            <m>\neg((\neg P \imp \neg Q) \wedge (\neg Q \imp R))</m>
            (careful with the implications).
          </li>

          <li>
            <p>
              For both parts above,
              verify your answers are correct using truth tables.
              That is, use a truth table to check that the given statement and your proposed simplification are actually logically equivalent.
            </p>
          </li>
        </ol>
      </p>
    </statement>
    <solution>
      <p>
        <ol>
          <li>
            <p>
              <m>\neg((\neg P \wedge Q) \vee \neg(R \vee \neg S))</m>
            </p>

            <p>
              <m>\neg(\neg P \wedge Q) \wedge \neg\neg(R \vee \neg S)</m> by De Morgan's law.
            </p>

            <p>
              <m>\neg(\neg P \wedge Q) \wedge (R \vee \neg S)</m> by double negation.
            </p>

            <p>
              <m>(\neg\neg P \vee \neg Q) \wedge (R \vee \neg S)</m> by De Morgan's law.
            </p>

            <p>
              <m>(P \vee \neg Q) \wedge (R \vee \neg S)</m> by double negation.
            </p>
          </li>

          <li>
            <p>
              We will need to convert the implications to disjunctions so we can apply De Morgan's law:
            </p>

            <p>
              <m>\neg((\neg P \imp \neg Q) \wedge (\neg Q \imp R))</m>
            </p>

            <p>
              <m>\neg((\neg \neg P \vee \neg Q) \wedge (\neg\neg Q \vee R))</m> by implication/disjunction equivalence.
            </p>

            <p>
              <m>\neg((P \vee \neg Q) \wedge (Q \vee R))</m> by double negation.
            </p>

            <p>
              <m>\neg(P \vee \neg Q) \vee \neg (Q \vee R)</m> by De Morgan's law.
            </p>

            <p>
              <m>(\neg P \wedge \neg \neg Q) \vee (\neg Q \wedge \neg R)</m> by De Morgan's law.
            </p>

            <p>
              <m>(\neg P \wedge Q) \vee (\neg Q \wedge \neg R)</m> by double negation.
            </p>
          </li>

          <li>
            <p>
              For each truth table,
              the columns for the original statement and the simplified statement must be identical.
              They are.
              For purposes of checking your work,
              here are the final columns for the two parts above:
            </p>

            <sidebyside width="60%">

              <tabular halign="center">
                <row bottom="medium">
                  <cell right="medium"><m>P</m></cell>
                  <cell right="medium"><m>Q</m></cell>
                  <cell right="medium"><m>R</m></cell>
                  <cell right="medium">(a)</cell>
                  <cell>(b)</cell>
                </row>
                <row>
                  <cell right="medium">T</cell>
                  <cell right="medium">T</cell>
                  <cell right="medium">T</cell>
                  <cell right="medium">T</cell>
                  <cell>F</cell>
                </row>
                <row>
                  <cell right="medium">T</cell>
                  <cell right="medium">T</cell>
                  <cell right="medium">F</cell>
                  <cell right="medium">F</cell>
                  <cell>F</cell>
                </row>
                <row>
                  <cell right="medium">T</cell>
                  <cell right="medium">F</cell>
                  <cell right="medium">T</cell>
                  <cell right="medium">T</cell>
                  <cell>F</cell>
                </row>
                <row>
                  <cell right="medium">T</cell>
                  <cell right="medium">F</cell>
                  <cell right="medium">F</cell>
                  <cell right="medium">T</cell>
                  <cell>T</cell>
                </row>
                <row>
                  <cell right="medium">F</cell>
                  <cell right="medium">T</cell>
                  <cell right="medium">T</cell>
                  <cell right="medium">F</cell>
                  <cell>T</cell>
                </row>
                <row>
                  <cell right="medium">F</cell>
                  <cell right="medium">T</cell>
                  <cell right="medium">F</cell>
                  <cell right="medium">F</cell>
                  <cell>T</cell>
                </row>
                <row>
                  <cell right="medium">F</cell>
                  <cell right="medium">F</cell>
                  <cell right="medium">T</cell>
                  <cell right="medium">T</cell>
                  <cell>F</cell>
                </row>
                <row>
                  <cell right="medium">F</cell>
                  <cell right="medium">F</cell>
                  <cell right="medium">F</cell>
                  <cell right="medium">T</cell>
                  <cell>T</cell>
                </row>
              </tabular>

            </sidebyside>

          </li>
        </ol>
      </p>
    </solution>
  </exercise>

  <exercise>
    <statement>
      <p>
        Consider the statement,
        <q>If a number is triangular or square, then it is not prime</q>

        <ol>
          <li>
            <p>
              Make a truth table for the statement <m>(T \vee S) \imp \neg P</m>.
            </p>
          </li>

          <li>
            <p>
              If you believed the statement was <em>false</em>,
              what properties would a counterexample need to possess?
              Explain by referencing your truth table.
            </p>
          </li>

          <li>
            <p>
              If the statement were true,
              what could you conclude about the number 5657, which is definitely prime?
              Again, explain using the truth table.
            </p>
          </li>
        </ol>
      </p>
    </statement>
    <solution>
      <p>
        <ol>
          <li>

            <sidebyside width="50%">

              <tabular halign="center">
                <row bottom="medium">
                  <cell right="medium"><m>T</m></cell>
                  <cell right="medium"><m>S</m></cell>
                  <cell right="medium"><m>P</m></cell>
                  <cell><m>(T\vee S) \imp \neg P</m></cell>
                </row>
                <row>
                  <cell right="medium">T</cell>
                  <cell right="medium">T</cell>
                  <cell right="medium">T</cell>
                  <cell>F</cell>
                </row>
                <row>
                  <cell right="medium">T</cell>
                  <cell right="medium">T</cell>
                  <cell right="medium">F</cell>
                  <cell>T</cell>
                </row>
                <row>
                  <cell right="medium">T</cell>
                  <cell right="medium">F</cell>
                  <cell right="medium">T</cell>
                  <cell>F</cell>
                </row>
                <row>
                  <cell right="medium">T</cell>
                  <cell right="medium">F</cell>
                  <cell right="medium">F</cell>
                  <cell>T</cell>
                </row>
                <row>
                  <cell right="medium">F</cell>
                  <cell right="medium">T</cell>
                  <cell right="medium">T</cell>
                  <cell>F</cell>
                </row>
                <row>
                  <cell right="medium">F</cell>
                  <cell right="medium">T</cell>
                  <cell right="medium">F</cell>
                  <cell>T</cell>
                </row>
                <row>
                  <cell right="medium">F</cell>
                  <cell right="medium">F</cell>
                  <cell right="medium">T</cell>
                  <cell>T</cell>
                </row>
                <row>
                  <cell right="medium">F</cell>
                  <cell right="medium">F</cell>
                  <cell right="medium">F</cell>
                  <cell>T</cell>
                </row>
              </tabular>

            </sidebyside>

          </li>

          <li>
            <p>
              There are three cases in which the statement is false:
              rows 1, 3 and 5.
              So one way to prove this was false would be to find a number that was triangular,
              square and prime
              (row 1).
              Or you could find a number that was triangular, not square,
              and prime (row 3) or one that is not triangular,
              is square and is not prime
              (row 5).
              In fact, since no square number is prime,
              we would need to do the second one (3 is both triangular and prime,
              but in fact this is the only one).
            </p>
          </li>

          <li>
            <p>
              Here we have a prime number,
              so we need to look at rows in which <m>P</m> is true.
              We also need to statement to be true.
              There is only one row with both these properties: row 7.
              And here we see that <m>T</m> and <m>S</m> are both false.
              So we would know that 5657 is neither triangular nor square.
            </p>
          </li>
        </ol>
      </p>
    </solution>
  </exercise>

  <exercise>
    <statement>
      <p>
        Tommy Flanagan was telling you what he ate yesterday afternoon.
        He tells you, <q>I had either popcorn or raisins.
        Also, if I had cucumber sandwiches, then I had soda.
        But I didn't drink soda or tea.</q>
        Of course you know that Tommy is the worlds worst liar,
        and everything he says is false.
        What did Tommy eat?
      </p>

      <p>
        Justify your answer by writing all of Tommy's statements using sentence variables (<m>P, Q, R, S, T</m>),
        taking their negations, and using these to deduce what Tommy actually ate.
      </p>
    </statement>
  </exercise>

  <exercise>
    <statement>
      <p>
        Determine if the following deduction rule is valid:
      </p>

      <sidebyside>

        <tabular halign="center">
          <row>
            <cell/>
            <cell><m>P \vee Q</m></cell>
          </row>
          <row bottom="minor">
            <cell/>
            <cell><m>\neg P</m></cell>
          </row>
          <row>
            <cell><m>\therefore</m></cell>
            <cell><m>Q</m></cell>
          </row>
        </tabular>

      </sidebyside>
    </statement>
    <solution>
      <p>
        The deduction rule is valid.
        To see this,
        make a truth table which contains <m>P \vee Q</m> and <m>\neg P</m>
        (and <m>P</m> and <m>Q</m> of course).
        Look at the truth value of <m>Q</m> in each of the rows that have
        <m>P \vee Q</m> and <m>\neg P</m> true.
      </p>
    </solution>
  </exercise>

  <exercise>
    <statement>
      <p>
        Determine if the following is a valid deduction rule:
      </p>

      <sidebyside>

        <tabular halign="center">
          <row>
            <cell/>
            <cell><m>P \imp (Q \vee R)</m></cell>
          </row>
          <row bottom="minor">
            <cell/>
            <cell><m>\neg(P \imp Q)</m></cell>
          </row>
          <row>
            <cell><m>\therefore</m></cell>
            <cell><m>R</m></cell>
          </row>
        </tabular>

      </sidebyside>
    </statement>
  </exercise>

  <exercise>
    <statement>
      <p>
        Determine if the following is a valid deduction rule:
      </p>

      <sidebyside>

        <tabular halign="center">
          <row>
            <cell/>
            <cell><m>(P \wedge Q) \imp R</m></cell>
          </row>
          <row bottom="minor">
            <cell/>
            <cell><m>\neg P \vee \neg Q</m></cell>
          </row>
          <row>
            <cell><m>\therefore</m></cell>
            <cell><m>\neg R</m></cell>
          </row>
        </tabular>

      </sidebyside>
    </statement>
  </exercise>

  <exercise>
    <statement>
      <p>
        Can you chain implications together?
        That is, if <m>P \imp Q</m> and <m>Q \imp R</m>,
        does that means the <m>P \imp R</m>?
        Can you chain more implications together?
        Let's find out:

        <ol>
          <li>
            <p>
              Prove that the following is a valid deduction rule:
            </p>

            <sidebyside>

              <tabular halign="center">
                <row>
                  <cell/>
                  <cell><m>P \imp Q</m></cell>
                </row>
                <row bottom="minor">
                  <cell/>
                  <cell><m>Q \imp R</m></cell>
                </row>
                <row>
                  <cell><m>\therefore</m></cell>
                  <cell><m>P \imp R</m></cell>
                </row>
              </tabular>

            </sidebyside>

          </li>

          <li>
            <p>
              Prove that the following is a valid deduction rule for any <m>n \ge 2</m>:
            </p>

            <sidebyside>

              <tabular halign="center">
                <row>
                  <cell/>
                  <cell><m>P_1 \imp P_2</m></cell>
                </row>
                <row>
                  <cell/>
                  <cell><m>P_2 \imp P_3</m></cell>
                </row>
                <row>
                  <cell/>
                  <cell><m>\vdots</m></cell>
                </row>
                <row bottom="minor">
                  <cell/>
                  <cell><m>P_{n-1} \imp P_n</m></cell>
                </row>
                <row>
                  <cell><m>\therefore</m></cell>
                  <cell><m>P_1 \imp P_n</m>.</cell>
                </row>
              </tabular>

            </sidebyside>

            <p>
              I suggest you don't go through the trouble of writing out a <m>2^n</m> row truth table.
              Instead, you should use part (a) and mathematical induction.
            </p>
          </li>
        </ol>
      </p>
    </statement>
  </exercise>

  <exercise>
    <statement>
      <p>
        We can also simplify statements in predicate logic using our rules for passing negations over quantifiers,
        and then applying propositional logical equivalence to the
        <q>inside</q> propositional part.
        Simplify the statements below
        (so negation appears only directly next to predicates).

        <ol>
          <li>
            <m>\neg \exists x \forall y (\neg O(x) \vee E(y))</m>.
          </li>

          <li>
            <m>\neg \forall x \neg \forall y \neg(x \lt y \wedge \exists z (x \lt z \vee y \lt z))</m>.
          </li>

          <li>
            <p>
              There is a number <m>n</m> for which no other number is either less <m>n</m> than or equal to <m>n</m>.
            </p>
          </li>

          <li>
            <p>
              It is false that for every number <m>n</m> there are two other numbers which <m>n</m> is between.
            </p>
          </li>
        </ol>
      </p>
    </statement>
    <solution>
      <p>
        <ol>
          <li>
            <m>\forall x \exists y (O(x) \wedge \neg E(y))</m>.
          </li>

          <li>
            <m>\exists x \forall y (x \ge y \vee \forall z (x \ge z \wedge y \ge z))</m>.
          </li>

          <li>
            <p>
              There is a number <m>n</m> for which every other number is strictly greater than <m>n</m>.
            </p>
          </li>

          <li>
            <p>
              There is a number <m>n</m> which is not between any other two numbers.
            </p>
          </li>
        </ol>
      </p>
    </solution>
  </exercise>

  <exercise>
    <statement>
      <p>
        Suppose <m>P</m> and <m>Q</m> are
        (possibly molecular)
        propositional statements.
        Prove that <m>P</m> and <m>Q</m> are logically equivalent if any only if <m>P \iff Q</m> is a tautology.
      </p>
    </statement>
    <hint>
      <p>
        What do these concepts mean in terms of truth tables?
      </p>
    </hint>
      <!-- TODO: needs solution -->
  </exercise>

  <exercise>
    <statement>
      <p>
        Suppose <m>P_1, P_2, \ldots, P_n</m> and <m>Q</m> are
        (possibly molecular)
        propositional statements.
        Suppose further that
      </p>

      <sidebyside>

        <tabular>
          <row>
            <cell/>
            <cell><m>P_1</m></cell>
          </row>
          <row>
            <cell/>
            <cell><m>P_2</m></cell>
          </row>
          <row>
            <cell/>
            <cell><m>\vdots</m></cell>
          </row>
          <row bottom="minor">
            <cell/>
            <cell><m>P_n</m></cell>
          </row>
          <row>
            <cell><m>\therefore</m></cell>
            <cell><m>Q</m></cell>
          </row>
        </tabular>

      </sidebyside>

      <p>
        is a valid deduction rule.
        Prove that the statement
        <me>
          (P_1 \wedge P_2 \wedge \cdots \wedge P_n) \imp Q
        </me>
        is a tautology.
      </p>
    </statement>
      <!-- TODO: needs solution -->
  </exercise>

</exercises>
