<?xml version="1.0" encoding="UTF-8"?>
<exercises permid="Jgi" xmlns:xi="http://www.w3.org/2001/XInclude" xml:id="exercises_seq-conc">
  <title>Chapter Review</title>
  <exercise permid="yen">
    <webwork>
        <statement>
          <p permid="WzT">
            Find <m>3 + 7 + 11+ \cdots + 427</m>.
          </p>

          <p permid="CHc">
            <var name="23005" width="5"/>
          </p>
        </statement>
        <solution permid="Ywk">
          <p permid="cpf">
            <m>\frac{430\cdot 107}{2} = 23005</m>.
          </p>
        </solution>
    </webwork>
  </exercise>

  <exercise permid="elw">
    <webwork>
        <setup>
          <pg-code>
            Context()->variables->are(n => "Real");
            $ans1 = Formula("n+2");
            $ans2 = Formula("4n+2");
            $ans3 = Formula("((4n+8)*(n+2))/2");
          </pg-code>
        </setup>
        <statement>
          <p permid="iOl">
            Consider the sequence <m>2, 6, 10, 14, \ldots, 4n + 6</m>.

            <ol permid="jFj">
              <li permid="sYV">
                <p permid="jjK">
                  How many terms are there in the sequence?
                </p>

                <p permid="PqT">
                  <var name="$ans1" width="10"/>
                </p>
              </li>

              <li permid="Zge">
                <p permid="vyc">
                  What is the second-to-last term?
                </p>

                <p permid="bFl">
                  <var name="$ans2" width="10"/>
                </p>
              </li>

              <li permid="Fnn">
                <p permid="HMu">
                  Find the sum of all the terms in the sequence.
                </p>

                <p permid="nTD">
                  <var name="$ans3" width="10"/>
                </p>
              </li>
            </ol>
          </p>
        </statement>
        <solution permid="EDt">
          <p permid="Iwo">
            <ol permid="mzP">
              <li permid="luw"><m>n+2</m> terms.</li>

              <li permid="RBF"><m>4n+2</m>.</li>

              <li permid="xIO"><m>\frac{(4n+8)(n+2)}{2}</m>.</li>
            </ol>
          </p>
        </solution>
    </webwork>
  </exercise>

  <exercise permid="KsF">
    <webwork>
        <setup>
          <pg-code>
            Context()->variables->are(n => "Real");
            $geometric = PopUp(
            ["?","arithmetic","geometric","neither"],
            "geometric", # correct answer
            );
            $sum = Compute("(2-2*5^25)/(-4)");
          </pg-code>
        </setup>
        <statement>
          <p permid="OVu">
            Consider the sequence given by <m>a_n = 2\cdot 5^{n-1}</m>.

            <ol permid="vTB">
              <li permid="dPX">
                <p permid="UaM">
                  Find the first 4 terms of the sequence.
                </p>
                <instruction>
                  <m>a_1 = </m> <var name="2" width="3"/>, <m>a_2 = </m> <var name="10" width="3"/>, <m>a_3 = </m> <var name="50" width="3"/>, <m>a_4 = </m> <var name="250" width="3"/> <ellipsis />.
                </instruction>
                <p permid="AhV">
                  What sort of sequence is this?
                </p>

                <p permid="gpe">
                  <var name="$geometric" form="popup"/>
                </p>
              </li>

              <li permid="JXg">
                <p permid="Mwn">
                  Find the <em>sum</em> of the first 25 terms.
                  That is, compute <m>\sum_{k=1}^{25}a_k</m>.
                </p>

                <p permid="sDw">
                  <var name="$sum" width="10"/>
                </p>
              </li>
            </ol>
          </p>
        </statement>
        <solution permid="kKC">
          <p permid="oDx">
            <ol permid="SGY">
              <li permid="qep">
                <m>2, 10, 50, 250, \ldots</m> The sequence is geometric.
              </li>

              <li permid="Wly"><m>\frac{2 - 2\cdot 5^{25}}{-4}</m>.</li>
            </ol>
          </p>
        </solution>
    </webwork>
  </exercise>

  <exercise permid="qzO">
    <statement>
      <p permid="vcD">
        Consider the sequence <m>5, 11, 19, 29, 41, 55,\ldots</m>.
        Assume <m>a_1 = 5</m>.

        <ol permid="caK">
          <li permid="CsH">
            <p permid="YKF">
              Find a closed formula for <m>a_n</m>,
              the <m>n</m>th term of the sequence,
              by writing each term as a sum of a sequence.
              Hint: first find <m>a_0</m>,
              but ignore it when collapsing the sum.
            <!-- <solution>
              <p>
                <m>a_0 = 1</m>, <m>a_1 = 1+4</m>, <m>a_2 = 1+4+6</m>, <m>a_3 = 1+4+6+8</m> and so on. If we ignore (for the moment) the 1, we have the sum of an arithmetic sequence. So
                <md>
                  <mrow> a_n \amp = 1 + [4 + 6 + 8 + 10 + \cdots + (2n) + (2+2n)]</mrow>
                  <mrow> + a_n \amp = 1 + [(2+2n) + (2n) + \cdots + 8 + 6 + 4]</mrow>
                  <mrow> \hline 2a_n \amp = 1 + n(2n+6)</mrow>
                </md>
              </p>

              <p>
                So <m>a_n = \frac{1+n(2n+6)}{2}</m>
            </p>
            </solution> -->
            </p>
          </li>

          <li permid="izQ">
            <p permid="ERO">
              Find a closed formula again,
              this time using either polynomial fitting or the characteristic root technique
              (whichever is appropriate).
              Show your work.
            <!-- <solution>
              <p>
                The sequence of first differences is <m>4, 6, 8, 10, 12,\ldots</m>, so the sequence of second differences is <m>2, 2, 2,\ldots</m> which is constant. Thus we know that the original sequence will be a quadratic: <m>a_n = an^2 + bn + c</m>. We know <m>a_0 = 1</m> so we have <m>c = 1</m>. This gives the system
                <me>
                  5 = a + b + 1
                </me>
            </p>
              <me>
                11 = 4a + 2 b + 1
              </me>
              <p>
                If we multiply the first equation by <m>-2</m> and add the second equation we get <m>1 = 2a - 1</m> so <m>a = 1</m>. Plugging this into the first equation gives <m>b = 3</m>. Thus the closed formula is <m>a_n = n^2 + 3n + 1</m>.
              </p>
            </solution> -->
            </p>
          </li>

          <li permid="OGZ">
            <p permid="kYX">
              Find a closed formula once again,
              this time by recognizing the sequence as a modification to some well known sequence(s).
              Explain.
            <!-- <solution>
              <p>
                If we compare our sequence to the sequence of squares <m>1,4,9, 16, 25,\ldots</m> we see a difference of <m>4, 7, 10, 13, 16, \ldots</m>. These are each 1 more than a multiple of 3. So we see that the sequence <m>5, 11, 19, 29, 41, 55,\ldots</m> is just the sequence of squares plus the sequence given by <m>3n+1</m>. So
                <me>
                  a_n = n^2 + 3n + 1
                </me>
            </p>
            </solution> -->
            </p>
          </li>
        </ol>
      </p>
    </statement>
  </exercise>

  <exercise permid="WGX">
    <webwork>
        <setup>
          <pg-code>
            Context()->variables->are(n => "Real");
            $ans = Formula("n^2 + 4n - 1");
          </pg-code>
        </setup>
        <statement>
          <p permid="bjM">
            Use polynomial fitting to find a closed formula for the sequence <m>(a_n)_{n\ge 1}</m>:
            <me permid="cYZ">
              4, 11, 20, 31, 44, \ldots
            </me>.
          </p>
          <instruction>
            <m>a_n = </m> <var name="$ans" width="10"/>
          </instruction>
        </statement>
        <solution permid="QRL">
          <p permid="UKG">
            <m>a_n = n^2 + 4n - 1</m>.
          </p>
        </solution>
    </webwork>
  </exercise>
      <!-- TODO: make multiple choice for webwork -->
  <exercise permid="COg">
    <statement>
      <p permid="HqV">
        Suppose the closed formula for a particular sequence is a degree 3 polynomial.
        What can you say about the closed formula for:

        <ol permid="IhT">
          <li permid="uOi">
            <p permid="Rgg">
              The sequence of partial sums.
            </p>
          </li>

          <li permid="aVr">
            <p permid="xnp">
              The sequence of second differences.
            </p>
          </li>
        </ol>
      </p>
    </statement>
    <solution permid="wYU">
      <p permid="ARP">
        <ol permid="yOh">
          <li permid="HcA">
            <p permid="duy">
              The sequence of partial sums will be a degree 4 polynomial
              (its sequence of differences will be the original sequence).
            </p>
          </li>

          <li permid="njJ">
            <p permid="JBH">
              The sequence of second differences will be a degree 1 polynomial - an arithmetic sequence.
            </p>
          </li>
        </ol>
      </p>
    </solution>
  </exercise>

  <exercise permid="iVp">
    <statement>
      <p permid="nye">
        Consider the sequence given recursively by <m>a_1 = 4</m>,
        <m>a_2 = 6</m> and <m>a_n = a_{n-1} + a_{n-2}</m>.

        <ol permid="opc">
          <li permid="TqS">
            <p permid="pIQ">
              Write out the first 6 terms of the sequence.
            </p>
          </li>

          <li permid="zyb">
            <p permid="VPZ">
              Could the closed formula for <m>a_n</m> be a polynomial?
              Explain.
            </p>
          </li>
        </ol>
      </p>
    </statement>
    <solution permid="dgd">
      <p permid="gYY">
        <ol permid="eVq">
          <li permid="fFk"><m>4, 6, 10, 16, 26, 42, \ldots</m>.</li>

          <li permid="LMt">
            <p permid="BXi">
              No, taking differences gives the original sequence back,
              so the differences will never be constant.
            </p>
          </li>
        </ol>
      </p>
    </solution>
  </exercise>

  <exercise permid="Pcy">
    <webwork>
        <setup>
          <pg-code>
            Context()->variables->are(n => "Real");
            $ans = Formula("(n+3)*n");
          </pg-code>
        </setup>
        <statement>
          <p permid="TFn">
            The sequence <m>(a_n)_{n \ge 1}</m> starts
            <m>-1, 0, 2, 5, 9, 14\ldots</m> and has closed formula <m>a_n = \dfrac{(n+1)(n-2)}{2}</m>.
            Use this fact to find a closed formula for the sequence
            <m>(b_n)_{n \ge 1}</m> which starts <m>4, 10, 18, 28, 40, \ldots</m>.
          </p>
          <instruction>
            <m>b_n = </m> <var name="$ans" width="10"/>
          </instruction>
        </statement>
        <solution permid="Jnm">
          <p permid="Ngh">
            <m>b_n = (n+3)n</m>.
          </p>
        </solution>
    </webwork>
  </exercise>

  <exercise permid="vjH">
    <statement>
      <p permid="zMw">
        The in song <em>The Twelve Days of Christmas</em>,
        my true love gave to me first 1 gift,
        then 2 gifts and 1 gift, then 3 gifts, 2 gifts and 1 gift,
        and so on.
        How many gifts did my true love give me all together during the twelve days?
      </p>
    </statement>
        <!-- TODO: needs solution -->
  </exercise>

  <exercise permid="bqQ">
    <webwork>
        <setup>
          <pg-code>
            Context()->variables->are(n => "Real");
            $ans = Formula("3/7 * (-2)^n + 4/7 * 5^n");
          </pg-code>
        </setup>
        <statement>
          <p permid="fTF">
            Consider the recurrence relation
            <m>a_n = 3a_{n-1} + 10 a_{n-2}</m> with first two terms <m>a_0 = 1</m> and <m>a_1 = 2</m>.

            <ol permid="Uwl">
              <li permid="rTC">
                <p permid="ier">
                  Write out the first 5 terms of the sequence defined by this recurrence relation.
                </p>
                <instruction>
                  <m>a_2 = </m> <var name="16" width="3"/>, <m>a_3 = </m> <var name="68" width="3"/>, <m>a_4 = </m> <var name="364" width="3"/>, <ellipsis />
                </instruction>
              </li>

              <li permid="YaL">
                <p permid="OlA">
                  Solve the recurrence relation.
                  That is, find a closed formula for <m>a_n</m>.
                </p>
                <instruction>
                  <m>a_n = </m> <var name="$ans" width="10"/>
                </instruction>
              </li>
            </ol>
          </p>
        </statement>
        <solution permid="puv">
          <p permid="tnq">
            <ol permid="Lcz">
              <li permid="EhU"><m>1, 2, 16, 68, 364, \ldots</m>.</li>

              <li permid="kpd"><m>a_n = \frac{3}{7}(-2)^n + \frac{4}{7}5^n</m>.</li>
            </ol>
          </p>
        </solution>
    </webwork>
  </exercise>

  <exercise permid="HxZ">
    <webwork>
        <setup>
          <pg-code>
            Context()->variables->are(n => "Real");
            $ans = Formula("1/6*(-2)^n + 5/6*4^n");
          </pg-code>
        </setup>
        <statement>
          <p permid="MaO">
            Consider the recurrence relation <m>a_n = 2a_{n-1} + 8a_{n-2}</m>,
            with initial terms <m>a_0 = 1</m> and <m>a_1= 3</m>.

            <ol permid="ADu">
              <li permid="Qwm">
                <p permid="usJ">
                  Find the next two terms of the sequence
                  (<m>a_2</m> and <m>a_3</m>).
                </p>
                <instruction>
                  <m>a_2 = </m> <var name="14" width="3"/>, <m>a_3 = </m> <var name="52" width="3"/>
                </instruction>
              </li>

              <li permid="wDv">
                <p permid="azS">
                  Solve the recurrence relation.
                  That is, find a closed formula for the <m>n</m>th term of the sequence.
                </p>
                <instruction>
                  <m>a_n = </m> <var name="$ans" width="10"/>
                </instruction>
              </li>
            </ol>
          </p>
        </statement>
        <solution permid="VBE">
          <p permid="Zuz">
            <ol permid="rjI">
              <li permid="cKE"><m>a_2 = 14</m>. <m>a_3 = 52</m>.</li>

              <li permid="IRN"><m>a_n = \frac{1}{6}(-2)^n + \frac{5}{6}4^n</m>.</li>
            </ol>
          </p>
        </solution>
    </webwork>
  </exercise>

  <exercise permid="nFi">
    <statement>
      <p permid="shX">
        Your magic chocolate bunnies
            <idx><h>magic chocolate bunnies</h></idx>
        reproduce like rabbits:
        every large bunny produces 2 new mini bunnies each day,
        and each day every mini bunny born the previous day grows into a large bunny.
        Assume you start with 2 mini bunnies and no bunny ever dies
        (or gets eaten).

        <ol permid="gKD">
          <li permid="oYW">
            <p permid="GHb">
              Write out the first few terms of the sequence.
            </p>
          </li>

          <li permid="Vgf">
            <p permid="mOk">
              Give a recursive definition of the sequence and explain why it is correct.
            </p>
          </li>

          <li permid="Bno">
            <p permid="SVt">
              Find a closed formula for the <m>n</m>th term of the sequence.
            </p>
          </li>
        </ol>
      </p>
    </statement>
    <solution permid="BIN">
      <p permid="lIR">
        <ol permid="XqR">
          <li permid="hux">
            <p permid="zcC">
              On the first day, your 2 mini bunnies become 2 large bunnies.
              On day 2, your two large bunnies produce 4 mini bunnies.
              On day 3, you have 4 mini bunnies
              (produced by your 2 large bunnies)
              plus 6 large bunnies
              (your original 2 plus the 4 newly matured bunnies).
              On day 4, you will have <m>12</m> mini bunnies (2 for each of the 6 large bunnies) plus 10 large bunnies
              (your previous 6 plus the 4 newly matured).
              The sequence of total bunnies is
              <m>2, 2, 6, 10, 22, 42\ldots</m> starting with <m>a_0 = 2</m> and <m>a_1 = 2</m>.
            </p>
          </li>

          <li permid="NBG">
            <m>a_n = a_{n-1} + 2a_{n-2}</m>.
            This is because the number of bunnies is equal to the number of bunnies you had the previous day
            (both mini and large)
            plus 2 times the number you had the day before that
            (since all bunnies you had 2 days ago are now large and producing 2 new bunnies each).
          </li>

          <li permid="tIP">
            <p permid="fjL">
              Using the characteristic root technique,
              we find <m>a_n = a2^n + b(-1)^n</m>,
              and we can find <m>a</m> and <m>b</m> to give <m>a_n = \frac{4}{3}2^n + \frac{2}{3}(-1)^n</m>.
            </p>
          </li>
        </ol>
      </p>
    </solution>
  </exercise>

  <exercise permid="TMr">
    <statement>
      <p permid="Ypg">
        Prove the following statements by mathematical induction:

        <ol permid="MRM">
          <li permid="ZPY"><m>n! \lt n^n</m> for <m>n \ge 2</m></li>

          <li permid="FXh">
            <m>\d\frac{1}{1\cdot 2} + \frac{1}{2\cdot 3} +\frac{1}{3\cdot 4}+\cdots + \frac{1}{n\cdot(n+1)} = \d\frac{n}{n+1}</m> for all <m>n \in \Z^+</m>.
          </li>

          <li permid="meq">
            <m>4^n - 1</m> is a multiple of 3 for all <m>n \in \N</m>.
          </li>

          <li permid="Slz">
            <p permid="LqU">
              The <em>greatest</em> amount of postage you <em>cannot</em>
              make exactly using 4 and 9 cent stamps is 23 cents.
            </p>
          </li>

          <li permid="ysI">
            <p permid="ryd">
              Every even number squared is divisible by 4.
            </p>
          </li>
        </ol>
      </p>
    </statement>
    <solution permid="hPW">
      <p permid="RQa">
        <ol permid="Dya">
          <li permid="ezR">
            <p permid="XFm">
              Hint: <m>(n+1)^{n+1} &gt; (n+1) \cdot n^{n}</m>.
            </p>
          </li>

          <li permid="KHa">
            <p permid="DMv">
              Hint: This should be similar to the other sum proofs.
              The last bit comes down to adding fractions.
            </p>
          </li>

          <li permid="qOj">
            <p permid="jTE">
              Hint: Write <m>4^{k+1} - 1 = 4\cdot 4^k - 4 + 3</m>.
            </p>
          </li>

          <li permid="WVs">
            <p permid="QaN">
              Hint: one 9-cent stamp is 1 more than two 4-cent stamps,
              and seven 4-cent stamps is 1 more than three 9-cent stamps.
            </p>
          </li>

          <li permid="DcB">
            <p permid="whW">
              Careful to actually use induction here.
              The base case: <m>2^2 = 4</m>.
              The inductive case:
              assume <m>(2n)^2</m> is divisible by 4 and consider <m>(2n+2)^2 = (2n)^2 + 4n + 4</m>.
              This is divisible by 4 because <m>4n +4</m> clearly is,
              and by our inductive hypothesis, so is <m>(2n)^2</m>.
            </p>
          </li>
        </ol>
      </p>
    </solution>
  </exercise>

  <exercise permid="zTA">
    <statement>
      <p permid="Ewp">
        Prove <m>1^3 + 2^3 + 3^3 + \cdots + n^3 = \left(\frac{n(n+1)}{2}\right)^2</m> holds for all <m>n \ge 1</m>,
        by mathematical induction.
      </p>
    </statement>
    <solution permid="NXf">
      <p permid="xXj">
        Hint: This is a straight forward induction proof.
        Note you will need to simplify
        <m>\left(\frac{n(n+1)}{2}\right)^2 + (n+1)^3</m> and get <m>\left(\frac{(n+1)(n+2)}{2}\right)^2</m>.
      </p>
    </solution>
  </exercise>

  <exercise permid="gaJ">
    <statement>
      <p permid="kDy">
        Suppose <m>a_0 = 1</m>,
        <m>a_1 = 1</m> and <m>a_n = 3a_{n-1} - 2a_{n-1}</m>.
        Prove, using strong induction,
        that <m>a_n = 1</m> for all <m>n</m>.
      </p>
    </statement>
    <solution permid="ueo">
      <p permid="ees">
        Hint: there are two base cases <m>P(0)</m> and <m>P(1)</m>.
        Then, for the inductive case,
        assume <m>P(k)</m> is true for all <m>k \lt n</m>.
        This allows you to assume <m>a_{n-1} = 1</m> and <m>a_{n-2} = 1</m>.
        Apply the recurrence relation.
      </p>
    </solution>
  </exercise>

  <exercise permid="MhS">
    <statement>
      <p permid="QKH">
        Prove, using strong induction,
        that every positive integer can be written as the sum of distinct powers of 2.
        For example, <m>13 = 1 + 4 + 8 = 2^0 + 2^2 + 2^3</m>.
      </p>
    </statement>
    <solution permid="alx">
      <p permid="KlB">
        Note that <m>1 = 2^0</m>; this is your base case.
        Now suppose <m>k</m> can be written as the sum of distinct powers of 2 for all <m>1\le k \le n</m>.
        We can then write <m>n</m> as the sum of distinct powers of 2 as follows:
        subtract the largest power of 2 less than <m>n</m> from <m>n</m>.
        That is, write <m>n = 2^j + k</m> for the largest possible <m>j</m>.
        But <m>k</m> is now less than <m>n</m>,
        and also less than <m>2^j</m>,
        so write <m>k</m> as the sum of distinct powers of 2
        (we can do so by the inductive hypothesis).
        Thus <m>n</m> can be written as the sum of distinct powers of 2 for all <m>n \ge 1</m>.
      </p>
    </solution>
  </exercise>

  <exercise permid="spb">
    <statement>
      <p permid="wRQ">
        Prove using induction that every set containing <m>n</m> elements has <m>2^n</m> different subsets for any <m>n \ge 1</m>.
      </p>
    </statement>
    <solution permid="GsG">
      <p permid="qsK">
        Let <m>P(n)</m> be the statement,
        <q>every set containing <m>n</m> elements has <m>2^n</m> different subsets.</q>
        We will show <m>P(n)</m> is true for all <m>n \ge 1</m>.

        <u>Base case</u>: Any set with 1 element <m>\{a\}</m> has exactly 2 subsets:
        the empty set and the set itself.
        Thus the number of subsets is <m>2= 2^1</m>.
        Thus <m>P(1)</m> is true.

        <u>Inductive case</u>: Suppose <m>P(k)</m> is true for some arbitrary <m>k \ge 1</m>.
        Thus every set containing exactly <m>k</m> elements has <m>2^k</m> different subsets.
        Now consider a set containing <m>k+1</m> elements:
        <m>A = \{a_1, a_2, \ldots, a_k, a_{k+1}\}</m>.
        Any subset of <m>A</m> must either contain <m>a_{k+1}</m> or not.
        In other words, a subset of <m>A</m> is just a subset of
        <m>\{a_1, a_2,\ldots,
        a_k\}</m> with or without <m>a_{k+1}</m>.
        Thus there are <m>2^k</m> subsets of <m>A</m> which contain <m>a_{k+1}</m> and another <m>2^{k+1}</m> subsets of <m>A</m> which do not contain <m>a^{k+1}</m>.
        This gives a total of <m>2^k + 2^k = 2\cdot 2^k = 2^{k+1}</m> subsets of <m>A</m>.
        But our choice of <m>A</m> was arbitrary,
        so this works for any subset containing <m>k+1</m> elements,
        so <m>P(k+1)</m> is true.
        Therefore, by the principle of mathematical induction,
        <m>P(n)</m> is true for all <m>n \ge 1</m>.
      </p>
    </solution>
  </exercise>

</exercises>
